thy/Bitmagic/Numberwang_Ln.thy
@@ -5,8 +5,8 @@ begin
 lemma ipv4range_bitmask_intersect: " \<not> ipv4range_set_from_bitmask b2 m2 \<subseteq> ipv4range_set_from_bitmask b1 m1 \<Longrightarrow>
        \<not> ipv4range_set_from_bitmask b1 m1 \<subseteq> ipv4range_set_from_bitmask b2 m2 \<Longrightarrow>
        ipv4range_set_from_bitmask b1 m1 \<inter> ipv4range_set_from_bitmask b2 m2 = {}"
-apply(simp add: ipv4range_set_from_bitmask_eq_ip_set)
-using ip_set_notsubset_empty_inter by presburger
+apply(simp add: ipv4range_set_from_bitmask_eq_ip4_set)
+using ip4_set_notsubset_empty_inter by presburger
 
 
 (*
